\documentclass[12pt]{article}
\usepackage{Packages}

\begin{document}

Two-country small open economy NK DSGE model for Scotland and the Rest of the UK.

\begin{enumerate}


    \item Home country: Scotland
    \item  Foreign country: RUK
    \item  Scotland and RUK are small and open economies
          \begin{enumerate}
              \item They take world output, inflation, and consumption as given and cannot influence it
          \end{enumerate}
    \item Scotland and RUK are assumed to be symmetrical in market structure and preferences
    \item Shocks in Scotland, RUK, and in the World Economy are assumed to be correlated
    \item Sticky nominal prices: Calvo Fairy
          \begin{enumerate}
              \item Here, I would prefer to use Rotemburg as it is more intuitive and less popular than Calvo Fairy
          \end{enumerate}
    \item For simplicity:
          \begin{enumerate}
              \item No nontradeable goods
              \item No trading costs
              \item No possibility of international policy coordination
              \item No cost-push shocks
              \item No nominal wage rigidities
              \item No international financial assetsa
          \end{enumerate}

\end{enumerate}

\pagebreak

\section{Households}
\subsection*{Consumer's problem}
A representative household wants to maximise the lifetime discounted utility:
\begin{equation}
    \E_0 \sum^{\infty}_{t=0} \left( \frac{C_t^{1-\sigma}}{1-\sigma} - \frac{N_t^{1+\varphi}}{1+\varphi} \right)
\end{equation}
Utility is is decreasingly increasing in consumption $C_t$ and decreasingly decreasing in hours worked $N_t$.

$C_t$ is a composite consumption index defined by
\begin{equation}
    C_t = \left[ (1-\alpha)^\frac{1}{\eta} (C_{H,t})^{\frac{\eta-1}{\eta}} + \alpha^{\frac{1}{\eta}}(C_{F,t})^{\frac{\eta-1}{\eta}}\right]^{\frac{\eta}{\eta-1}}
\end{equation}
\begin{align}
    C_{H,t} & = \left( \int_{0}^{1} {C_{H,t}(j)}^{\frac{\varepsilon-1}{\varepsilon}} \,dj  \right)^\frac{\varepsilon}{\varepsilon-1} & \text{ Index of consumption of home produced goods}                 \\
    C_{i,t} & = \left( \int_{0}^{1} {C_{i,t}(j)}^{\frac{\varepsilon-1}{\varepsilon}} \,dj  \right)^\frac{\varepsilon}{\varepsilon-1} & \text{ Index of consumption of country \textit{i}'s produced goods} \\
    C_{F,t} & = \left( \int_{0}^{1} {C_{i,t}}^{\frac{\gamma-1}{\gamma}} \,di  \right)^{\frac{\gamma}{\gamma-1}}                      & \text{ Index of consumption of imported goods}
\end{align}

Optimal allocation of each variety of goods:
\begin{align}
    C_{H,t}(j) & = \left( \frac{P_{H,t}(j)}{P_{H,t}}\right)^{-\varepsilon}C_{H,t}; & C_{i,t}(j) & = \left( \frac{P_{i,t}(j)}{P_{i,t}}\right)^{-\varepsilon}C_{i,t}; & C_{i,t} & = \left( \frac{P_{i,t}}{P_{F,t}}\right)^{-\gamma}C_{F,t}\label{eq:optimal_imported_consumption}
\end{align}
\begin{align}
    P_{H,t} & = \left( \int_{0}^{1} P_{H,t}(j)^{1-\varepsilon} \,dj  \right)^{\frac{1}{1-\varepsilon}}                                  & \text{Domestic Price Index}                                \\
    P_{i,t} & = \left( \int_{0}^{1} P_{i,t}(j)^{1-\varepsilon} \,dj  \right)^{\frac{1}{1-\varepsilon}}                                  & \text{Price Index of goods produced by country \textit{i}} \\
    P_{F,t} & = \left( \int_{0}^{1} P_{i,t}^{1-\gamma} \,dj  \right)^{\frac{1}{1-\gamma}}         \label{eq:price_index_imported_goods} & \text{Price Index of Imported goods}
\end{align}
\begin{align}
    \int_{0}^{1} & P_{H,t}(j)C_{H,t}(j) \,dj = P_{H,t}C_{H,t} & \int_{0}^{1} & P_{i,t}(j)C_{i,t}(j) \,dj = P_{i,t}C_{i,t}
\end{align}
Using (\ref{eq:optimal_imported_consumption}) and (\ref{eq:price_index_imported_goods}) implies
\begin{equation}
    \int_{0}^{1} P_{i,t}C_{i,t} = P_{F,t}C_{F,t}
\end{equation}
\begin{align}
    C_{H,t} & = (1-\alpha) {\left(\frac{P_{H,t}}{P_t}\right)}^{-\eta} C_{t} & C_{F,t} & = \alpha {\left(\frac{P_{F,t}}{P_t}\right)}^{-\eta} C_{t}
\end{align}
\begin{align}
    P_t = \left[ (1-\alpha) (P_{H,t})^{1-\eta} + \alpha (P_{F,t})^{1-\eta} \right]^{\frac{1}{1-\eta}} &  & \text{ Consumption Price Index}
\end{align}
A special case $\eta=1$:
\begin{align}
    P_t & = (P_{H,t})^{1-\alpha} \times (P_{F,t})^{\alpha} & C_t & = \frac{1}{(1-\alpha)^{(1-\alpha)}\alpha^\alpha}(C_{H,t})^{(1-\alpha)}(C_{F,t})^\alpha
\end{align}
Total consumption expenditures are:
\begin{align}
    P_{H,t}C_{H,t} + P_{F,t}C_{F,t} = P_t C_t
\end{align}
So the budget constraint is:
\begin{align}
    P_t C_t + \E_t [Q_{t,t+1}D_{t+1}] \leq D_t + W_t N_t + T_t
\end{align}
\begin{align}
    \mathcal{L} & = \E_0 \sum^{\infty}_{t=0} \left( \frac{C_t^{1-\sigma}}{1-\sigma} - \frac{N_t^{1+\varphi}}{1+\varphi} \right)  \nonumber \\ &+ \lambda_t\left\{  D_t + W_t N_t + T_t - P_t C_t - \E_t [Q_{t,t+1}D_{t+1}] \right\}
\end{align}
\begin{align*}
    \frac{\partial L}{\partial C_t}                                    & = \beta^t C_t^{-\sigma} - \lambda_t P_t = 0; \quad \Rightarrow \quad \beta^t C_t^{-\sigma} P_{t}^{-1} = \lambda_t  \\
    \frac{\partial L}{\partial N_t}                                    & = -\beta^t N_t^{\varphi} + \lambda_t N_t = 0; \quad \Rightarrow \quad \beta^t N_t^{\varphi} W_{t}^{-1} = \lambda_t \\
    \frac{\partial L}{\partial C_t} = \frac{\partial L}{\partial N_t}: & \beta^t C_t^{-\sigma} P_{t}^{-1} = \beta^t N_t^{\varphi} W_{t}^{-1}                                                \\
    \Rightarrow                                                        & C_t^{-\sigma} P_{t}^{-1} = N_t^{\varphi} W_{t}^{-1}                                                                \\
    \Rightarrow                                                        & C_t^{-\sigma} N_t^{-\varphi} =  W_{t}^{-1}     P_{t}
\end{align*}
\begin{align}
    \Rightarrow &  & C_t^{\sigma} N_t^{\varphi} =  \frac{W_t}{P_t} \label{eq:intratemporal_optimality_condition} &  & \text{Intratemporal Optimality Condition}
\end{align}
\begin{align*}
    \frac{\partial L}{\partial C_t}     & = \beta^t C_t^{-\sigma} P_{t}^{-1} = \lambda_t; \quad \Rightarrow \quad \E_t[\beta^{t+1} C_{t+1}^{-\sigma} P_{t+1}^{-1}] = \E_t[\lambda_{t+1}] \\
    \frac{\partial L}{\partial D_{t+1}} & = -\lambda_t \E_t[Q_{t,t+1}] + \E_t[\lambda_{t+1}] = 0; \quad \Rightarrow \quad \E_t[Q_{t,t+1}] = \frac{\lambda_{t+1}}{\lambda_t}
\end{align*}
\begin{align*}
    \E_t\left[\frac{\beta^t C_t^{-\sigma} P_{t}^{-1}}{\beta^{t+1} C_{t+1}^{-\sigma} P_{t+1}^{-1}}\right]                 & = \E_t\left[\frac{\lambda_t}{\lambda_{t+1}}\right] \\
    \E_t\left[\frac{\beta^t C_t^{-\sigma} P_{t}^{-1}}{\beta^{t+1} C_{t+1}^{-\sigma} P_{t+1}^{-1}}\right]                 & = \E_t\left[\frac{1}{Q_{t,t+1}}\right]             \\
    \E_t\left[\frac{1}{\beta} \left(\frac{C_t}{C_{t+1}}\right)^{-\sigma} \left(\frac{P_{t}}{ P_{t+1}}\right)^{-1}\right] & = \E_t\left[\frac{1}{Q_{t,t+1}}\right]
\end{align*}
\begin{align}
    \beta\E_t\left[\left(\frac{C_{t+1}}{C_{t}}\right)^{-\sigma} \left(\frac{P_{t}}{ P_{t+1}}\right)\right]                 = Q_t &  & \text{Euler equation}
\end{align}
However, Gali uses a different approach to derive the Euler equation, which introduces Arrow securities:
\begin{equation}
    \frac{V_{t,t+1}}{P_t}C_{t}^{-\sigma} = \xi_{t,t+1} \beta C_{t+1}^{-\sigma} \frac{1}{P_{t+1}} \label{eq:introduces_arrow_securities}
\end{equation}
Where $V_{t,t+1}$ is an Arrow security and $\xi_{t,t+1}$ is the probability that the Arrow security will yield a payoff next period. Interpretation: LHS is paying for the security (expenses) in terms of consumption at $P_t$ prices. RHS is the payoff if the Arrow security yields a payoff. The consumer will only be willing to pay LHS if the payoff is at least as big on the RHS.
Given that:
\begin{equation}
    Q_{t,t+1} = \frac{V_{t,t+1}}{\xi_{t,t+1}}
\end{equation}
\begin{align}
    \frac{V_{t,t+1}}{P_t}C_{t}^{-\sigma} = \xi_{t,t+1} \beta C_{t+1}^{-\sigma} \frac{1}{P_{t+1}} \\
    Q_{t,t+1} = \beta \left(\frac{C_{t+1}}{C_{t}}\right)^{-\sigma} \frac{P_t}{P_{t+1}}           \\
    \E_t [Q_{t,t+1}] = \beta \E_t\left[\left(\frac{C_{t+1}}{C_{t}}\right)^{-\sigma} \frac{P_t}{P_{t+1}}\right]
\end{align}
\begin{align}
    \beta\E_t\left[\left(\frac{C_{t+1}}{C_{t}}\right)^{-\sigma} \left(\frac{P_{t}}{ P_{t+1}}\right)\right] \label{eq:euler_equation}                = Q_t &  & \text{Euler equation}
\end{align}
Log-linearising (\ref{eq:intratemporal_optimality_condition}):
\begin{align}
    C_t^{\sigma} N_t^{\varphi} =  \frac{W_t}{P_t}; \quad \Rightarrow \quad w_t - p_t = \sigma c_t + \varphi n_t
\end{align}
Log-linearising (\ref{eq:euler_equation}):
\begin{align}
    \beta\E_t\left[\left(\frac{C_{t+1}}{C_{t}}\right)^{-\sigma} \left(\frac{P_{t}}{ P_{t+1}}\right)\right]                = Q_t \nonumber \\
    \ln\beta - \E_t[\sigma c_{t+1}] + \sigma c_t + p_t - \E_t [p_{t+1}] = \ln Q_t                                              \nonumber  \\
    \sigma c_t  = \ln Q_t - \ln \beta + \E_t[\sigma c_{t+1}] - p_t + \E_t [p_{t+1}]                                             \nonumber \\
    c_t =  \E_t[c_{t+1}] - \frac{1}{\sigma}( -\ln Q_t - \rho - \E_t [\pi_{t+1}]   )                                             \nonumber \\
    c_t =  \E_t[c_{t+1}] - \frac{1}{\sigma}( i_t  - \E_t [\pi_{t+1}] - \rho  )                                                            \\
    \text{where $i_t = -\log Q_t$, $\rho = -\log \beta$, $\pi_t = p_t - p_{t-1}$} \nonumber
\end{align}
\begin{align}
    S_{i,t} = \frac{P_{i,t}}{P_{H,t}}                                                                                                     &  & \text{Bilateral terms of trade}       \\
    S_{t} =  \frac{P_{F,t}}{P_{H,t}} = \left(\int_{0}^{1} (S_{i,t} \, di)^{1-\gamma}\right)^{\frac{1}{1-\gamma}}                          &  & \text{Effective terms of trade}       \\
    s_t = p_{F,t} - p_{H,t} = \left(\int_{0}^{1} s_{i,t} \, di \right)                                      \label{eq:terms_of_trade_log} &  & \text{(log) Effective terms of trade}
\end{align}
Recall that when $\eta = 1$, then CPI is $P_t = (P_{H,t})^{1-\alpha} \times (P_{F,t})^{\alpha}$, which can be log-linearised to:
\begin{equation}
    p_t = (1-\alpha)p_{H,t} + \alpha p_{F,t} = p_{H,t} + \alpha s_t \label{eq:domestic_price_plus_bilateral_terms_of_trade}
\end{equation}
Equations (\ref{eq:terms_of_trade_log}) and (\ref{eq:domestic_price_plus_bilateral_terms_of_trade}) hold when $\gamma=1$ and $\eta = 1$, respectively.
\begin{align}
    \pi_{H,t} = p_{H,t+1} - p_{H,t}         &  & \text{Domestic Inflation} \\
    \pi_{t} = \pi_{H,t} + \alpha \Delta s_t &  & \text{CPI Inflation}
\end{align}
The gap between domestic inflation and CPI inflation is only due to percentage change in the terms of trade.
\begin{align}
    P_{i,t}(j) & = \mathcal{E}_{i,t}P_{i,t}^i(j)                                                                         &  & \text{Law of One Price (LOP)}              \\
    P_{i,t}    & = \mathcal{E}_{i,t}P_{i,t}^i                                                                            &  & \text{Law of One Price (LOP)}              \\
    p_{i,t}    & = e_{i,t}+p_{i,t}^i                                                                                     &  & \text{(Log) Law of One Price (LOP)}        \\
    p_{F,t}    & = \int_{0}^{1}(e_{i,t}+p_{i,t}^i) \,di = e_t + p_t^{\star} \label{eq:log_price_index_of_imported_goods} &  & \text{(Log )Price index of Imported Goods}
\end{align}
Where $e_t$ is (Log) Effective Nominal Exchange Rate, $p_t^{\star}$ is the World Price Index.
\begin{align}
    s_t = p_{F,t} - p_{H,t} = e_t + p_t^{\star} - p_{H,t} \label{eq:terms_of_trade_with_world_price_index} &  & \text{Terms of trade but with the World Price Index}
\end{align}
\begin{align}
    \mathcal{Q}_{i,t} & = \frac{\mathcal{E}_{i,t}P_{t}^i}{P_t}                                        &  & \text{Bilateral Exchange Rate}                                       \\
    q_t               & = \int_{0}^{1} \log \left( \frac{\mathcal{E}_{i,t}P_{t}^i}{P_t} \right) \, di                                                                           \\
                      & = \int_{0}^{1} (e_{i,t} + p_{i,t}^i - p_t) \, di                              &  &                                                                      \\
                      & = e_t + p_t^{\star} - p_t                                                     &  & \text{using (\ref{eq:log_price_index_of_imported_goods})}            \\
                      & = s_t + p_{H_t} - p_t                                                         &  & \text{using (\ref{eq:terms_of_trade_with_world_price_index})}        \\
                      & = (1-\alpha)s_t                                                               &  & \text{using (\ref{eq:domestic_price_plus_bilateral_terms_of_trade})}
\end{align}
International Risk-Sharing
Equation (\ref{eq:introduces_arrow_securities}) for country \textit{i} can be rewritten as:
\begin{align}
    \frac{V_{t,t+1}}{\mathcal{E}^i_tP^i_t}({C^{i}_{t}})^{-\sigma} = \xi_{t,t+1} \beta ({C^{i}_{t+1}})^{-\sigma} \frac{1}{\mathcal{E}^i_{t+1}P^{i}_{t+1}}
\end{align}
Given that:
\begin{equation}
    Q_{t,t+1} = \frac{V_{t,t+1}}{\xi_{t,t+1}}
\end{equation}
\begin{align}
    \frac{V_{t,t+1}}{\mathcal{E}^i_tP^i_t}({C^{i}_{t}})^{-\sigma}                                                                                           & = \xi_{t,t+1} \beta ({C^{i}_{t+1}})^{-\sigma} \frac{1}{\mathcal{E}^i_{t+1}P^{i}_{t+1}}                                                                    \\
    Q_{t,t+1}                                                                                                                                               & = \beta \left(\frac{C^i_{t+1}}{C^i_{t}}\right)^{-\sigma} \left(\frac{P^i_t}{P^i_{t+1}}\right) \left(\frac{\mathcal{E}^i_{t}}{\mathcal{E}^i_{t+1}} \right) \\
    Q_{t,t+1}                                                                                                                                               & = \beta \left(\frac{C_{t+1}}{C_{t}}\right)^{-\sigma} \frac{P_t}{P_{t+1}}  \text{ using Equation (XX)}                                                     \\
    \beta \left(\frac{C^i_{t+1}}{C^i_{t}}\right)^{-\sigma} \left(\frac{P^i_t}{P^i_{t+1}}\right) \left(\frac{\mathcal{E}^i_{t}}{\mathcal{E}^i_{t+1}} \right) & = \beta \left(\frac{C_{t+1}}{C_{t}}\right)^{-\sigma} \frac{P_t}{P_{t+1}}                                                                                  \\
    \left(\frac{C^i_{t+1}}{C^i_{t}}\right)^{-\sigma} \left(\frac{P^i_t}{P^i_{t+1}}\right) \left(\frac{\mathcal{E}^i_{t}}{\mathcal{E}^i_{t+1}} \right)       & = \left(\frac{C_{t+1}}{C_{t}}\right)^{-\sigma} \frac{P_t}{P_{t+1}}                                                                                        \\
    \left(\frac{C^i_{t}}{C^i_{t+1}}\right)^{\sigma} \left(\frac{P^i_t}{P^i_{t+1}}\right) \left(\frac{\mathcal{E}^i_{t}}{\mathcal{E}^i_{t+1}} \right)        & = \left(\frac{C_{t}}{C_{t+1}}\right)^{\sigma} \frac{P_t}{P_{t+1}}                                                                                         \\
    {C^{i}_{t}}^{\sigma} P_t^i \mathcal{E}_t^i                                                                                                              & = C_t^{\sigma} P_t                                                                                                                                        \\
    {C^{i}_{t}}^{\sigma}                                                                                                                                    & = C_t^{\sigma} \frac{1}{\mathcal{Q}_{i,t}}                                                                                                                \\
    C_t = C^i_t \mathcal{Q}_{i,t}^{\frac{1}{\sigma}} \label{eq:domestic_consumption_and_real_exchange_rate}
\end{align}
Log-linearising (\ref{eq:domestic_consumption_and_real_exchange_rate}) yields:
\begin{equation}
    c_t = c_{t}^i + \frac{1}{\sigma}q_{i,t}
\end{equation}
Integrating both sides over \textit{i}:
\begin{align}
    c_t & = c_t^{\star} + \frac{1}{\sigma}q_t                                                                               &  &                                  \\
        & = c_t^{\star} + \left(\frac{1-\alpha}{\sigma}\right)s_t \label{eq:link_between_consumption_and_world_consumption} &  & \text{using $q_t=(1-\alpha)s_t$}
\end{align}
$c_t^{\star}$ is the log world consumption. Equation (\ref{eq:link_between_consumption_and_world_consumption}) is the link between the domestic consumption and the world consumption.
\section{Firms}
\begin{align}
    Y_t(j)   & = A_t N_t(j)                          \\
    \log A_t & = \alpha_t                            \\
    \alpha_t & = \rho_a \alpha_{t-1} + \varepsilon_t
\end{align}
\begin{align}
    L             & =P_{t}(j)Y_{t}(j) - W_t(j)N_{t}(j) \\
    \Rightarrow L & =P_{t}Y_{t} - W_tN_{t}             \\
    \Rightarrow L & =P_{t}A_t N_t - W_tN_{t}           \\
\end{align}
\begin{align}
    \frac{\partial L}{\partial N_t} & = P_t A_t - W_t = 0          &  & \Rightarrow W_t - P_tA_t = 0 \\
    MC_t                            & = W_t - P_tA_t                                                 \\
    mc_t                            & = w_t - p_t - a_t                                              \\
    mc_t                            & = -\nu + w_t - p_t - a_t                                       \\
    mc_t                            & = -\nu + w_t - p_{H,t} - a_t                                   \\
\end{align}
$\nu=-(\log (1-\tau))$, where $\tau$ is the employment subsidy, introduced later. $p_{H,t}$ because this is for domestic firms.

Firms that get to reset their price, do it using the following problem:
\begin{equation}
    \bar{p_{H,t}} = \mu + (1-\beta \theta) \sum_{k=0}^{\infty} (\beta \theta)^{k} \E_t [mc_{t+k} + p_{H,t+k}]
\end{equation}
\begin{align}
    \bar{p_{H,t}} &  & \text{Is the (log) new price}                  \\
    \mu           &  & \text{Is the (log) markup in the steady state}
\end{align}
\section{Equilibrium}
\begin{align}
    Y_t(j) & = C_{H,t}(j) + \int_{0}^{1} C_{H,t}^i (j) \, di                                                                                                                                                                                                                                      \\
           & =\left(\frac{P_{H,t}(j)}{P_{H,t}}^{-\varepsilon}\right) \left[ (1-\alpha) \left(\frac{P_{H,t}}{P_t} \right)^{-\eta} C_t + \alpha \int_{0}^{1} \left( \frac{P_{H_t}}{\mathcal{E}_{i,t}P_{F,t}^i}\right)^{-\gamma} \left(\frac{P_{F,t}^i}{P_t^i} \right)^{-\eta} C_{t}^i \, di \right]
\end{align}
Given that
\begin{equation}
    Y_t = \left( \int_{0}^{1} (Y_t(j))^{\frac{\varepsilon-1}{\varepsilon}}\right)^{\frac{\varepsilon}{\varepsilon-1}}
\end{equation}
\begin{align}
    Y_t & = (1-\alpha) \left(\frac{P_{H,t}}{P_t} \right)^{-\eta} C_t + \alpha \int_{0}^{1} \left( \frac{P_{H_t}}{\mathcal{E}_{i,t}P_{F,t}^i}\right)^{-\gamma} \left(\frac{P_{F,t}^i}{P_t^i} \right)^{-\eta} C_{t}^i \, di \\
        & = \left(\frac{P_{H,t}}{P_t}\right)^{-\eta}C_t \left[ (1-\alpha) + \alpha \int_{0}^{1} (S_t^i S_{i,t})^{\gamma - \eta} \mathcal{Q}_{i,t}^{\eta - \frac{1}{\sigma}} \, di \right]
\end{align}
Which can be log-linearised to:
\begin{align}
    y_t & = c_t + \alpha \gamma s_t + \alpha(\eta - \frac{1}{\sigma})q_t \\
        & = c_t + \frac{\alpha w}{\sigma}s_t                             \\
    w_t & = \sigma \gamma + (1-\alpha)(\sigma \eta - 1)
\end{align}
Assuming that country \textit{i} is symmetric:
\begin{align}
    y_t^i = c_t^i + \frac{\alpha w}{\sigma} s_t^i            &  &                          \\
    \int_{0}^{1} y_t^i = \int_{0}^{1} c_t^i + 0 =c_t^{\star} &  & \text{World Consumption}
\end{align}
Using equations (), (), ():
\begin{align}
    y                     & = c_t + \frac{\alpha w}{\sigma}s_t                                       \\
    y_t                   & = c_t^{\star} + \frac{1-\alpha}{\sigma}s_t + \frac{\alpha w}{\sigma} s_t \\
    y_t                   & = y_t^{\star} + \frac{1-\alpha}{\sigma}s_t + \frac{\alpha w}{\sigma} s_t \\
    y_t                   & = y_t^{\star} + \frac{1-\alpha + \alpha w}{\sigma}s_t                    \\
    y_t                   & = y_t^{\star} + \frac{1+ \alpha(w-1)}{\sigma}s_t                         \\
    \sigma_\alpha         & = \frac{1+ \alpha(w-1)}{\sigma}                                          \\
    \Rightarrow \quad y_t & =y^{\star}_t + \frac{1}{\sigma_\alpha}s_t
\end{align}
\end{document}