\newgeometry{left=0.5cm,bottom=1cm,right=0.5cm,top=1cm}

\renewcommand{\arraystretch}{10}
\begin{table}[H]
    \centering
    \begin{tabular}{l|l c}
    \makecell{Scenario 1 \\ (G: 2, $\tau: 0$)} &  \makecell{S HBC: \\ rUK HBC: \\ S GBC: \\ rUK GBC: \\ S TR: \\ rUK TR: \\ S Debt s.:\\ rUK Debt s.:\\ S Bonds: \\ rUK Bonds: \\ S RC: \\ rUK RC:} & 
        \makecell{
            $P_t C_t + \E_t [{R^{-1}_{t+1}}B_{t+1}] = B_t + W_t N_t + T_t$ \\
            $P^*_t C^*_t + \E_t [{R^{*-1}_{t+1}}B^*_{t+1}] = B^*_t + W^*_t N^*_t + T^*_t$ \\
            $\E_t [{R^{-1}_{t+1}}B_{t+1}] + T_t = P_tG_t + B_t$\\
            $\E_t [{R^{*-1}_{t+1}}B^*_{t+1}] + T^*_t = P^*_tG^*_t + B^*_t$ \\
            $T_t = P_tG_t$ \\
            $T^*_t = P_tG^*_t$ \\
            $T_t / P_t = \phi^*_g G_Y g_t + \phi^*_b(B_t / P_t); \quad G_Y = 0$\\
            $T^*_t / P^*_t = \phi^*_g G^*_Y g^*_t + \phi^*_b(B^*_t / P^*_t); \quad G_Y = 0$\\
            $(B_{t+1} / P_t) / R_{t+1} = (1-\phi_g) G_Y g_t + (1-\phi_b)(B_t / P_t); \quad G_Y = 0$\\
            $(B^*_{t+1} / P^*_t) / R^*_{t+1} = (1-\phi^*_g) G^*_Y g^*_t + (1-\phi^*_b)(B^*_t / P^*_t); \quad G^*_Y = 0$\\
            $Y_t = C_t + G_t + X_t$ \\
            $Y^*_t = C^*_t + G^*_t + X^*_t$
        }  \\ 
    \makecell{Scenario 2 \\ (G: 1, $\tau: 0$)} &  \makecell{S HBC: \\ rUK HBC: \\ S GBC: \\ rUK GBC: \\ S TR: \\ rUK TR:\\ S Debt s.:\\ rUK Debt s.:\\ S Bonds: \\ rUK Bonds: \\ S RC: \\ rUK RC:} & 
        \makecell{
            $P_t C_t + \E_t [{R^{UK-1}_{t+1}}B^{UK}_{t+1}] = B^{UK}_t + W_t N_t + \varpi T^{UK}_t$ \\
            $P^*_t C^*_t + \E_t [{R^{UK-1}_{t+1}}B^{UK}_{t+1}] = B^{UK}_t + W^*_t N^*_t + (1-\varpi)T^{UK}_t$ \\
            N/A\\
            $\E_t [{R^{UK-1}_{t+1}}B^{UK}_{t+1}] + T^{UK}_t = P^{UK}_tG^{UK}_t + B^{UK}_t$\\
            N/A \\
            $T^{UK}_t = P^{UK}_tG^{UK}_t$ \\
            N/A\\
            $T^{UK}_t / P^{UK}_t = \phi^{UK}_g G^{UK}_Y g^{UK}_t + \phi^{UK}_b(B^{UK}_{t+1} / P^{UK}_t); \quad G^{UK}_Y = 0$\\
            N/A\\
            $(B^{UK}_t / P^{UK}_t) / R^{UK}_{t+1} = (1-\phi^{UK}_g) G^{UK}_Y g^{UK}_t + (1-\phi^{UK}_b)(B^{UK}_t / P^{UK}_t); \quad G^{UK}_Y = 0$\\
            $Y_t = C_t + \varpi G^{UK}_t + X_t$ \\
            $Y^*_t = C^*_t + (1-\varpi) G^{UK}_t + X^*_t$
        }   \\ 
    \makecell{Scenario 3 \\ (G: 2, $\tau: 1$)} &  \makecell{S HBC: \\ rUK HBC: \\ S GBC: \\ rUK GBC: \\ S TR: \\ rUK TR: \\ S Debt s.:\\ rUK Debt s.:\\ S Bonds: \\ rUK Bonds: \\ S RC: \\ rUK RC:} & 
    \makecell{
        $P_t C_t + \E_t [{R^{-1}_{t+1}}B_{t+1}] = B_t + (1-\tau_t)W_t N_t + T_t$ \\
        $P^*_t C^*_t + \E_t [{R^{*-1}_{t+1}}B^*_{t+1}] = B^*_t + (1-\tau^*_t)W^*_t N^*_t + T^*_t$ \\
        $\E_t [{R^{-1}_{t+1}}B_{t+1}] + T_t = P_tG_t + B_t$\\ 
        $\E_t [{R^{*-1}_{t+1}}B^*_{t+1}] + T^*_t = P^*_tG^*_t + B^*_t$\\ 
        $T_t = \tau_t W_t N_t$ \\
        $T^*_t = \tau^*_t W^*_t N^*_t$ \\
        $T_t / P_t = \phi^*_g G_Y g_t + \phi^*_b(B_t / P_t); \quad G_Y = \tau$\\
        $T^*_t / P^*_t = \phi^*_g G^*_Y g^*_t + \phi^*_b(B^*_t / P^*_t); \quad G_Y = \tau^*$\\
        $(B_{t+1} / P_t) / R_{t+1} = (1-\phi_g) G_Y g_t + (1-\phi_b)(B_t / P_t); \quad G_Y = \tau$\\
        $(B^*_{t+1} / P^*_t) / R^*_{t+1} = (1-\phi^*_g) G^*_Y g^*_t + (1-\phi^*_b)(B^*_t / P^*_t); \quad G^*_Y = \tau^*$\\
        $Y_t = C_t + G_t + X_t$ \\
        $Y^*_t = C^*_t + G^*_t + X^*_t$
    }  \\
    \makecell{Scenario 4 \\ (G: 1, $\tau: 1$)} &  \makecell{S HBC: \\ rUK HBC: \\ S GBC: \\ rUK GBC: \\ S TR: \\ rUK TR: \\ S Debt s.:\\ rUK Debt s.:\\ S Bonds: \\ rUK Bonds: \\ S RC: \\ rUK RC:} & 
    \makecell{
        $P_t C_t + \E_t [{R^{UK-1}_{t+1}}B^{UK}_{t+1}] = B^{UK}_t + (1-\tau^{UK}_t)W_t N_t + \varpi T^{UK}_t$ \\
        $P^*_t C^*_t + \E_t [{R^{UK-1}_{t+1}}B^{UK}_{t+1}] = B^{UK}_t + (1-\tau^{UK}_t)W^*_t N^*_t + (1-\varpi)T^{UK}_t$ \\
        N/A \\
        $\E_t [{R^{UK-1}_{t+1}}B^{UK}_{t+1}] + T^{UK}_t = P^{UK}_tG^{UK}_t + B^{UK}_t$\\ 
        N/A \\
        $T^{UK}_t = \varpi\tau^{UK}_t W_t N_t + (1-\varpi)\tau^{UK}_t W^*_t N^*_t$ \\
        N/A\\
        $T^{UK}_t / P^{UK}_t = \phi^{UK}_g G^{UK}_Y g^{UK}_t + \phi^{UK}_b(B^{UK}_t / P^{UK}_t); \quad G^{UK}_Y = \tau^{UK}$\\
        N/A\\
        $(B^{UK}_{t+1} / P^{UK}_t) / R^{UK}_{t+1} = (1-\phi^{UK}_g) G^{UK}_Y g^{UK}_t + (1-\phi^{UK}_b)(B^{UK}_t / P^{UK}_t); \quad G^{UK}_Y = \tau^{UK}$\\
        $Y_t = C_t + \varpi G^{UK}_t$ \\
        $Y^*_t = C^*_t + (1-\varpi) G^{UK}_t$
    }  
    \end{tabular}
    \end{table}
where:
\begin{table}[H]
    \centering
    \begin{tabular}{c|c}
        \makecell{
            S HBC \\
            rUK HBC \\
            S GBC \\
            rUK GBC \\
            S TR \\
            rUK TR \\
            S RC \\
            rUK RC \\
        } & 
        \makecell{
            Household (Scotland) budget constraint \\
            Household (rUK) budget constraint \\
            Government (Holyrood) budget constraint \\
            Government (Westminister) budget constraint \\
            Government (Holyrood) tax revenue \\
            Government (Westminister) tax revenue \\
            Resource (Scotland) constraint \\
            Resource (rUK) constraint \\
        }
    \end{tabular}
\end{table}

\restoregeometry

\renewcommand{\arraystretch}{2}

\begin{table}[H]
    \centering
    \begin{tabular}{l|l|c}
    \makecell{Scenario 1 \\ (G: 2, $\tau: 0$)} & \makecell{Scotland \\ rUK } & 
        \makecell{
            $P_t C_t + \E_t [{R^{-1}_{t+1}}B_{t+1}] = B_t + W_t N_t + T_t$ \\
            $P^*_t C^*_t + \E_t [{R^{*-1}_{t+1}}B^*_{t+1}] = B^*_t + W^*_t N^*_t + T^*_t$
        }  \\ 
    \makecell{Scenario 2 \\ (G: 1, $\tau: 0$)} & \makecell{Scotland \\ rUK } & 
        \makecell{
            $P_t C_t + \E_t [{R^{UK-1}_{t+1}}B^{UK}_{t+1}] = B^{UK}_t + W_t N_t + \varpi T^{UK}_t$ \\
            $P^*_t C^*_t + \E_t [{R^{UK-1}_{t+1}}B^{UK}_{t+1}] = B^{UK}_t + W^*_t N^*_t + (1-\varpi)T^{UK}_t$
        }   \\ 
    \makecell{Scenario 3 \\ (G: 2, $\tau: 1$)} & \makecell{Scotland \\ rUK } & 
    \makecell{
        $P_t C_t + \E_t [{R^{-1}_{t+1}}B_{t+1}] = B_t + (1-\tau_t)W_t N_t + T_t$ \\
        $P^*_t C^*_t + \E_t [{R^{*-1}_{t+1}}B^*_{t+1}] = B^*_t + (1-\tau^*_t)W^*_t N^*_t + T^*_t$ 
    }  \\
    \makecell{Scenario 4 \\ (G: 1, $\tau: 1$)} & \makecell{Scotland \\ rUK } & 
    \makecell{
        $P_t C_t + \E_t [{R^{UK-1}_{t+1}}B^{UK}_{t+1}] = B^{UK}_t + (1-\tau^{UK}_t)W_t N_t + \varpi T^{UK}_t$ \\
        $P^*_t C^*_t + \E_t [{R^{UK-1}_{t+1}}B^{UK}_{t+1}] = B^{UK}_t + (1-\tau^{UK}_t)W^*_t N^*_t + (1-\varpi)T^{UK}_t$
    }  
    \end{tabular}
    \end{table}