\subsubsection{Derivation of loglinearised aggregate resource constraint}
\begin{align}\label{eq:appendix_log_rc_beginning}
    Y_t &= (1-\upsilon)\left(\frac{P_{H,t}}{P_t}\right)^{-\eta}C_t + \upsilon \mathcal{S}_t^{\eta}Y_t^* + G_t\\
    Y \mathbf{e}^{y_t} &= (1-\upsilon)\left(\frac{P}{P_{H}}\right)^{\eta}C \mathbf{e}^{-\eta p_{H,t} + \eta p_t + c_t}+ \upsilon S^{\eta} Y^* \mathbf{e}^{\eta s_t + y^*_t} + G \mathbf{e}^{g_t}\\
    Y ({1+y_t}) &= (1-\upsilon)\left(\frac{P}{P_{H}}\right)^{\eta}C ({1 -\eta p_{H,t} + \eta p_t + c_t})+ \upsilon S^{\eta} Y^* ({1 + \eta s_t + y^*_t}) + G ({1+ g_t})\\
    Y y_t &= (1-\upsilon)\left(\frac{P}{P_{H}}\right)^{\eta}C ({-\eta p_{H,t} + \eta p_t + c_t})+ \upsilon S^{\eta} Y^* ({\eta s_t + y^*_t}) + G g_t\\
    &\text{Using $P/P_H = \mathcal{S}^\upsilon$, $\mathcal{S} = 1$, and $C=Y^*$}:\nonumber\\
    y_t &= C_Y\left[(1-\upsilon)({-\eta p_{H,t} + \eta p_t + c_t})+ \upsilon ({\eta s_t + y^*_t})\right] + G_Y g_t\\
    &\text{Using $p_t - p_{H,t} = \upsilon s_t$}:\nonumber\\
    y_t &= C_Y\left[(1-\upsilon)({\eta \upsilon s_t + c_t})+ \upsilon ({\eta s_t + y^*_t})\right] + G_Y g_t\\
    y_t &= C_Y\left[(1-\upsilon)c_t + (1-\upsilon) \eta \upsilon s_t + \upsilon {\eta s_t} + \upsilon y^*_t\right] + G_Y g_t\\
    y_t &= C_Y\left[(1-\upsilon)c_t + \upsilon (2-\upsilon)\eta s_t + \upsilon y^*_t\right] + G_Y g_t \label{eq:appendix_log_rc_end}
\end{align}
\newpage