\subsubsection*{Derivation of natural real interest rate}
\tiny
\begin{align}\label{eq:appendix_natural_real_interest_rate_beginning}
    r^n_t  &= C_Y^{-1}\sigma_\upsilon \E_t \{\Delta y^n_{t+1}\} + \rho + \sigma_\upsilon \upsilon (\varpi - 1)\E \{\Delta y_{t+1}^* \}  + \Phi (1-\upsilon)(1-\rho_z)z_t - \sigma_\upsilon C_G^{-1}\E_t \{ \Delta g_{t+1} \}\\
    C_Y^{-1} \sigma_\upsilon \E_t\{\Delta y^n_{t+1}\} &= C_Y^{-1} \sigma_\upsilon \E_t\{\Gamma_* \Delta y^*_{t+1} + \Gamma_z \Delta z_{t+1} + \Gamma_a \Delta a_{t+1} + \Gamma_g \Delta g_{t+1} + \Gamma_\tau \Delta \tau_{t+1}\}\\
    &\text{Consider each term in turn:}\nonumber\\
    y^*_t&: C_Y^{-1} \sigma_\upsilon \Gamma_* \Delta y^*_{t+1} + \sigma_\upsilon \upsilon(\varpi-1)\Delta y^*_{t+1} = \sigma_\upsilon(C_Y^{-1} \Gamma_* + \upsilon(\varpi-1))\Delta y^*_{t+1} = \Psi_* \E_t \{\Delta y^*_{t+1}\}\\
    z_t&: C_Y^{-1} \sigma_\upsilon \Gamma_z \Delta z_{t+1} + \Phi (1-\upsilon) (1-\rho_z)z_t = C_Y^{-1} \sigma_\upsilon \Gamma_z (\rho_z - 1)z_t + \Phi (1-\upsilon)(1-\rho_z)z_t\\
    &= C_Y^{-1} \sigma_\upsilon \Gamma_z (\rho_z - 1)z_t + \Phi (1-\upsilon)(1-\rho_z)z_t = ((1-\upsilon)\Phi - C_Y^{-1} \sigma_\upsilon \Gamma_z)(1-\rho_z)z_t = \Psi_z (1-\rho_z) z_t\\
    a_t&: C_Y^{-1} \sigma_\upsilon \Gamma_a \Delta a_{t+1} = C_Y^{-1} \sigma_\upsilon \Gamma_a (\rho_a - 1)a_t = - C_Y^{-1} \sigma_\upsilon \Gamma_a (1 - \rho_a)a_t\\
    g_t&: C_Y^{-1} \sigma_\upsilon \Gamma_g \Delta g_{t+1} - \sigma_\upsilon C_G^{-1}\E_t \{ \Delta g_{t+1} \}  = \left( \sigma_\upsilon \left( C_Y^{-1} \Gamma_g - C_G^{-1} \right)\right) \E_t \{ \Delta g_{t+1}\} = -\Psi_g (1-\rho_g)g_t\\
    \tau_t&: \sigma_\upsilon C_Y^{-1} \Gamma_\tau \Delta \tau_{t+1} = \Psi_\tau \E_t \{ \Delta \tau_{t+1}\}\\
    &\text{Finally:}\nonumber\\
    r^n_t  &= \rho - C_Y^{-1} \sigma_\upsilon \Gamma_a (1 - \rho_a)a_t + \Psi_* \E_t \{\Delta y^*_{t+1}\} + \Psi_z (1-\rho_z) z_t - \Psi_g (1-\rho_g)g_t +\Psi_\tau \E_t \{ \Delta \tau_{t+1}\}
\end{align}
where:
\begin{align}
    \Psi_* &= \sigma_\upsilon(C_Y^{-1} \Gamma_* + \upsilon(\varpi-1)) \\
    \Psi_z &= (1-\upsilon)\Phi - C_Y^{-1} \sigma_\upsilon \Gamma_z \\
    \Psi_g &= \sigma_\upsilon \left( C_Y^{-1} \Gamma_g - C_G^{-1} \right)\\
    \Psi_\tau &= \sigma_\upsilon C_Y^{-1} \Gamma_\tau \label{eq:appendix_natural_real_interest_rate_end}
\end{align}
\newpage