International Risk-Sharing Equation for country \textit{i} can be rewritten as:
\begin{align}
    \frac{V_{t,t+1}}{\mathcal{E}^i_tP^i_t}({C^{i}_{t}})^{-\sigma} = \xi_{t,t+1} \beta ({C^{i}_{t+1}})^{-\sigma} \frac{1}{\mathcal{E}^i_{t+1}P^{i}_{t+1}}
\end{align}
Given that:
\begin{equation}
    Q_{t,t+1} = \frac{V_{t,t+1}}{\xi_{t,t+1}}
\end{equation}
\begin{align}
    \frac{V_{t,t+1}}{\mathcal{E}^i_tP^i_t}({C^{i}_{t}})^{-\sigma}         & = \xi_{t,t+1} \beta ({C^{i}_{t+1}})^{-\sigma} \frac{1}{\mathcal{E}^i_{t+1}P^{i}_{t+1}}                                                                    \\
    Q_{t,t+1}                                                             & = \beta \left(\frac{C^i_{t+1}}{C^i_{t}}\right)^{-\sigma} \left(\frac{P^i_t}{P^i_{t+1}}\right) \left(\frac{\mathcal{E}^i_{t}}{\mathcal{E}^i_{t+1}} \right) 
\end{align}
Recall that:
\begin{align}
    \frac{\partial L}{\partial C_t} &= \beta^t C_t^{-\sigma} P_{t}^{-1} = \lambda_t \nonumber\\
    \frac{\partial L}{\partial D_{t+1}} & = -\lambda_t \E_t[Q_{t,t+1}] = -\E_t[\lambda_{t+1}] \nonumber\\
    &=-\beta^t C_t^{-\sigma} P_{t}^{-1} \E_t[Q_{t,t+1}] = -\E_t[\lambda_{t+1}] \label{eq:derivative_c_t_home_country}
\end{align}
Which is symmetrical for country \textit{i}:
\begin{align}
    \frac{\partial L^i}{\partial C_t^i} &= \beta^t {(C^i_t)}^{-\sigma} (\mathcal{E}_{i,t}P^i_{t})^{-1} = \lambda^i_t \nonumber\\
    \frac{\partial L^i}{\partial D_{t+1}^i} & = -\lambda^i_t \E_t[Q_{t,t+1}] = -\E_t[\lambda^i_{t+1}] \nonumber\\
    &=-\beta^t {(C^i_t)}^{-\sigma} (\mathcal{E}_{i,t}P^i_{t})^{-1} \E_t[Q_{t,t+1}] = -\E_t[\lambda^i_{t+1}] \label{eq:derivative_c_t_i_country}
\end{align}
\begin{align*}
    \frac{\text{(\ref{eq:derivative_c_t_home_country})}}{\text{(\ref{eq:derivative_c_t_i_country})}}: \frac{-\beta^t C_t^{-\sigma} P_{t}^{-1} \E_t[Q_{t,t+1}]}{-\beta^t {(C^i_t)}^{-\sigma} (\mathcal{E}_{i,t}P^i_{t})^{-1} \E_t[Q_{t,t+1}]} &= \frac{-\E_t[\lambda_{t+1}]}{-\E_t[\lambda^i_{t+1}]}
\end{align*} 
\begin{align*}   
    C_t^{-\sigma}{(C^i_t)}^{\sigma} \frac{\mathcal{E}_{i,t}P^i_{t}}{P_t} &= 1 \\
    C_t^{-\sigma}{(C^i_t)}^{\sigma} \mathcal{Q}_{i,t} &= 1 \\
    C_t^{-\sigma}{(C^i_t)}^{\sigma}  &= \frac{1}{\mathcal{Q}_{i,t}} \\
    C_t^{-\sigma}  &= \frac{1}{\mathcal{Q}_{i,t}}{(C^i_t)}^{-\sigma} \\
    C_t^{\sigma}  &= \mathcal{Q}_{i,t}{(C^i_t)}^{\sigma}
\end{align*}
\begin{equation}
    \Rightarrow C_t  = {C^i_t}\mathcal{Q}_{i,t}^{\frac{1}{\sigma}}
\end{equation}